refact: compatibility lam

CollapsingTowers/TwoLvLBasic/Syntax/Closedness.lean
@@ -22,6 +22,38 @@ def closed_at (e : Expr) (x : ℕ) : Prop :=
 @[simp]
 def closed e := closed_at e 0
 
+-- closedness condition for bound variables
+@[simp]
+def lc_at (e : Expr) (i : ℕ) : Prop :=
+  match e with
+  | .bvar j => j < i
+  | .fvar _ => true
+  | .lam e => lc_at e (i + 1)
+  | .lift e => lc_at e i
+  | .app₁ f arg => lc_at f i ∧ lc_at arg i
+  | .app₂ f arg => lc_at f i ∧ lc_at arg i
+  | .lit _ => true
+  | .run e => lc_at e i
+  | .code e => lc_at e i
+  | .reflect e => lc_at e i
+  | .lam𝕔 e => lc_at e (i + 1)
+  | .lets b e => lc_at b i ∧ lc_at e (i + 1)
+  | .lets𝕔 b e => lc_at b i ∧ lc_at e (i + 1)
+
+@[simp]
+def lc e := lc_at e 0
+
+@[simp]
+def wf_at (e : Expr) (x : ℕ) : Prop := lc e ∧ closed_at e x
+
+@[simp]
+def wf (e : Expr) : Prop := wf_at e 0
+
+@[simp]
+def multi_wf : Subst → Prop
+  | [] => true
+  | v :: γ => wf v ∧ multi_wf γ
+
 lemma closed.fv_not_in_dec :
   ∀ e x,
     closed_at e (x + 1) →
@@ -280,6 +312,16 @@ lemma closed.under_erase : ∀ e x, closed_at e x ↔ closed_at ‖e‖ x :=
   | lam𝕔 _ IH =>
     apply IH
 
+lemma closed.under_multi_subst : ∀ γ e, multi_wf γ → closed_at e γ.length → closed (multi_subst γ e) :=
+  by
+  intros γ e Hγ He
+  induction γ generalizing e
+  case nil => apply He
+  case cons IH =>
+    apply IH; apply Hγ.right
+    apply closed.under_subst_dec; apply closed.inc
+    apply Hγ.left.right; omega; apply He
+
 lemma closed_impl_fv_not_in :
   ∀ x y e,
     closed_at e x →
@@ -337,3 +379,125 @@ lemma closed_iff_fv_empty : ∀ e, closed e ↔ fv e = (∅ : Set ℕ) :=
       simp; constructor
       apply IH₀.mpr; apply Hclosed.left
       apply IH₁.mpr; apply Hclosed.right
+
+lemma lc.inc:
+  ∀ e i j,
+    lc_at e i → i ≤ j →
+    lc_at e j :=
+  by
+  intros e i j Hclosed HLe
+  induction e generalizing i j with
+  | bvar => simp at *; omega
+  | fvar => simp
+  | lam _ IH
+  | lift _ IH
+  | lam𝕔 _ IH
+  | code _ IH
+  | reflect _ IH
+  | run _ IH =>
+    apply IH; apply Hclosed; omega
+  | app₁ _ _ IH₀ IH₁
+  | app₂ _ _ IH₀ IH₁
+  | lets _ _ IH₀ IH₁
+  | lets𝕔 _ _ IH₀ IH₁ =>
+    apply And.intro
+    . apply IH₀; apply Hclosed.left; omega
+    . apply IH₁; apply Hclosed.right; omega
+  | lit => simp
+
+lemma lc.under_opening : ∀ i x e, lc_at ({i ↦ x} e) i ↔ lc_at e (i + 1) :=
+  by
+  intros i x e
+  induction e generalizing i with
+  | bvar j =>
+    by_cases HEq : j = i
+    . simp [if_pos HEq]; omega
+    . simp [if_neg HEq]; omega
+  | fvar => simp
+  | lit => simp
+  | lam _ IH
+  | lift _ IH
+  | lam𝕔 _ IH
+  | code _ IH
+  | reflect _ IH
+  | run _ IH =>
+    apply IH
+  | app₁ _ _ IH₀ IH₁
+  | app₂ _ _ IH₀ IH₁
+  | lets _ _ IH₀ IH₁
+  | lets𝕔 _ _ IH₀ IH₁ =>
+    constructor
+    . intro Hlc
+      constructor
+      apply (IH₀ _).mp; apply Hlc.left
+      apply (IH₁ _).mp; apply Hlc.right
+    . intro Hlc
+      constructor
+      apply (IH₀ _).mpr; apply Hlc.left
+      apply (IH₁ _).mpr; apply Hlc.right
+
+lemma lc.under_closing : ∀ e x i j, j < i → lc_at e i → lc_at ({j ↤ x} e) i :=
+  by
+  intros e x i j Hlt
+  induction e generalizing i j with
+  | fvar y =>
+    by_cases HEq : x = y
+    . rw [HEq]; simp; omega
+    . simp; rw [if_neg HEq]; simp
+  | bvar => simp
+  | lam _ IH
+  | lift _ IH
+  | lam𝕔 _ IH
+  | code _ IH
+  | reflect _ IH
+  | run _ IH =>
+    apply IH; omega
+  | app₁ _ _ IH₀ IH₁
+  | app₂ _ _ IH₀ IH₁
+  | lets _ _ IH₀ IH₁
+  | lets𝕔 _ _ IH₀ IH₁ =>
+    intro Hlc; constructor
+    apply IH₀; omega; apply Hlc.left
+    apply IH₁; omega; apply Hlc.right
+  | lit => simp
+
+lemma lc.under_subst : ∀ x e v i, lc_at v i → lc_at e i → lc_at (subst x v e) i :=
+  by
+  intros x e v i Hv He
+  induction e generalizing i with
+  | bvar => apply He
+  | fvar y =>
+    by_cases HEq : x = y
+    . rw [HEq]; simp; apply Hv
+    . simp; rw [if_neg HEq]; simp
+  | lam _ IH
+  | lift _ IH
+  | lam𝕔 _ IH =>
+    apply IH; apply lc.inc
+    apply Hv; omega; apply He
+  | app₁ _ _ IH₀ IH₁
+  | app₂ _ _ IH₀ IH₁ =>
+    constructor
+    apply IH₀; apply Hv; apply He.left
+    apply IH₁; apply Hv; apply He.right
+  | lets _ _ IHb IH
+  | lets𝕔 _ _ IHb IH =>
+    constructor
+    apply IHb; apply Hv; apply He.left
+    apply IH; apply lc.inc
+    apply Hv; omega; apply He.right
+  | code _ IH
+  | reflect _ IH
+  | run _ IH =>
+    simp; apply IH; apply Hv; apply He
+  | lit => simp
+
+lemma lc.under_multi_subst : ∀ i γ e, multi_wf γ → lc_at e i → lc_at (multi_subst γ e) i :=
+  by
+  intros i γ e Hγ He
+  induction γ generalizing e
+  case nil => apply He
+  case cons IH =>
+    apply IH; apply Hγ.right
+    apply lc.under_subst; apply lc.inc
+    apply Hγ.left.left; omega; apply He
