CollapsingTowers/TwoLvLBasic/Syntax/Wf.lean
@@ -1,8 +1,0 @@
-import CollapsingTowers.TwoLvLBasic.Syntax.Lc
-import CollapsingTowers.TwoLvLBasic.Syntax.Closed
-
-@[simp]
-def wf_at (e : Expr) (x : ℕ) : Prop := lc e ∧ closed_at e x
-
-@[simp]
-def wf (e : Expr) : Prop := wf_at e 0
