CollapsingTowers/TwoLvLBasic/LogicEquiv/Defs.lean
@@ -1,3 +1,4 @@
 import CollapsingTowers.TwoLvLBasic.LogicEquiv.LogicRelation
 import CollapsingTowers.TwoLvLBasic.LogicEquiv.Symmetry
 import CollapsingTowers.TwoLvLBasic.LogicEquiv.Transitive
+import CollapsingTowers.TwoLvLBasic.LogicEquiv.Compatibility
