CollapsingTowers/TwoLvLBasic/Syntax/Commutative.lean
@@ -1,7 +1,6 @@
 import CollapsingTowers.TwoLvLBasic.Syntax.Identity
 
-lemma comm.subst_opening :
-    ∀ x y v e i, x ≠ y → lc v → subst x v ({i ↦ y} e) = ({i ↦ y} subst x v e) :=
+lemma comm.subst_opening : ∀ x y v e i, x ≠ y → lc v → subst x v ({i ↦ y} e) = ({i ↦ y} subst x v e) :=
   by
   intro x y v e i HNe Hlc
   induction e generalizing i with
@@ -34,8 +33,7 @@ lemma comm.subst_opening :
   | lam𝕔 _ IH =>
     simp; apply IH
 
-lemma comm.shiftl_opening :
-    ∀ x y e n i, x ≤ y → (shiftl_at x n {i ↦ y} e) = ({i ↦ y + n} shiftl_at x n e) :=
+lemma comm.shiftl_opening : ∀ x y e n i, x ≤ y → (shiftl_at x n {i ↦ y} e) = ({i ↦ y + n} shiftl_at x n e) :=
   by
   intros x y e n i HLe
   induction e generalizing i with
@@ -61,8 +59,7 @@ lemma comm.shiftl_opening :
   | run _ IH =>
     simp; apply IH
 
-lemma comm.shiftr_opening :
-    ∀ x y e i, x < y → shiftr_at x (opening i (.fvar y) e) = opening i (.fvar (y - 1)) (shiftr_at x e) :=
+lemma comm.shiftr_opening : ∀ x y e i, x < y → shiftr_at x (opening i (.fvar y) e) = opening i (.fvar (y - 1)) (shiftr_at x e) :=
   by
   intros x y e i HLe
   induction e generalizing i with
@@ -109,3 +106,60 @@ lemma comm.erase_opening : ∀ i x e, ‖{i ↦ x} e‖ = {i ↦ x} ‖e‖ :=
   | run _ IH
   | lam _ IH
   | lam𝕔 _ IH => simp; apply IH
+
+lemma comm.multi_subst_opening : ∀ γ x e i, x ≥ γ.length → multi_wf γ → multi_subst γ ({i ↦ x} e) = {i ↦ x} (multi_subst γ e) :=
+  by
+  intros γ x e i HGe Hγ
+  induction γ generalizing e
+  case nil => rfl
+  case cons IH =>
+    simp at *
+    rw [comm.subst_opening, IH]
+    omega; apply Hγ.right; omega
+    apply lc.inc; apply Hγ.left.left; omega
+
+lemma comm.subst_subst : ∀ x y v₀ v₁ e, x ≠ y → closed v₀ → closed v₁ → subst x v₀ (subst y v₁ e) = subst y v₁ (subst x v₀ e) :=
+  by
+  intro x y v₀ v₁ e HNe Hclose₀ Hclose₁
+  induction e with
+  | bvar j => simp
+  | fvar z =>
+    by_cases HEqx : x = z
+    . simp [if_pos HEqx]
+      by_cases HEqy : y = z
+      . simp [if_pos HEqy]
+        omega
+      . simp [if_neg HEqy, if_pos HEqx]
+        rw [identity.subst]
+        apply closed.inc; apply Hclose₀; omega
+    . simp [if_neg HEqx]
+      by_cases HEqy : y = z
+      . simp [if_pos HEqy]
+        rw [identity.subst]
+        apply closed.inc; apply Hclose₁; omega
+      . simp [if_neg HEqy, if_neg HEqx]
+  | app₁ _ _ IH₀ IH₁
+  | app₂ _ _ IH₀ IH₁
+  | lets _ _ IH₀ IH₁
+  | lets𝕔 _ _ IH₀ IH₁ =>
+    simp; constructor
+    apply IH₀; apply IH₁
+  | lam _ IH
+  | lift _ IH
+  | lam𝕔 _ IH
+  | code _ IH
+  | reflect _ IH
+  | run _ IH =>
+    simp; apply IH
+  | lit => simp
+
+lemma comm.multi_subst_subst : ∀ x γ v e, x ≥ γ.length → closed v →  multi_wf γ → subst x v (multi_subst γ e) = multi_subst γ (subst x v e) :=
+  by
+  intro x γ v e HGe Hclose Hγ
+  induction γ generalizing e
+  case nil => simp
+  case cons IH =>
+    simp at HGe
+    rw [multi_subst, multi_subst, IH, comm.subst_subst]
+    omega; apply Hclose; apply Hγ.left.right
+    omega; apply Hγ.right
